Regex/Notation.lean
@@ -1,0 +1,149 @@
+import Regex.Regex
+
+namespace Regex.Notation
+
+/-!
+## Notation
+
+Notation `regex%` to build the regular expression at compile time.
+-/
+
+open Lean
+
+def toNumLit (n : Nat) : NumLit := Lean.Syntax.mkNumLit (ToString.toString n)
+
+theorem eq_true_of_decide_ext (p : Prop) (inst : Decidable p) (h : decide p = true) : p = True :=
+  @eq_true_of_decide p inst h
+
+theorem of_eq_true_ext (p : Prop) (h : p = True) : p :=
+  @of_eq_true p h
+
+/-- proof of `n` < `m`
+
+  for example
+
+  @of_eq_true (1 < 300)
+    (@eq_true_of_decide (1 < 300) (Nat.decLt 1 300) (of_decide_eq_true (Eq.refl true)))
+  : 1 < 300
+
+-/
+private def mkTermOfDecideLt (n m : Nat) : Term :=
+  let eq_refl : Term := Syntax.mkApp (mkCIdent `Eq.refl) #[Quote.quote true]
+  let of_decide_eq_true := Syntax.mkApp (mkCIdent ``of_decide_eq_true) #[eq_refl]
+  let decLt := Syntax.mkApp (mkCIdent `Nat.decLt) #[toNumLit n, toNumLit m]
+  let lt_lt := Syntax.mkApp (mkCIdent `LT.lt) #[toNumLit n, toNumLit m]
+  let eq_true_of_decide := Syntax.mkApp (mkCIdent ``eq_true_of_decide_ext)
+                            #[lt_lt, decLt, of_decide_eq_true]
+  Syntax.mkApp (mkCIdent ``of_eq_true_ext) #[lt_lt, eq_true_of_decide]
+
+private def mkTermOfFin (f: Fin n) : Term :=
+  Syntax.mkApp (mkCIdent ``Fin.mk)
+                #[Syntax.mkNumLit (ToString.toString f.val), mkTermOfDecideLt f.val n]
+
+instance : Quote (Fin n) where
+  quote := mkTermOfFin
+
+private def mkTermOfUInt32 (n : UInt32) : Term :=
+  Syntax.mkApp (mkCIdent `UInt32.mk) #[Quote.quote n.val]
+
+instance : Quote UInt32 where
+  quote := mkTermOfUInt32
+
+private def mkTermOfTransition (t: NFA.Checked.Transition n) : Term :=
+  Syntax.mkApp (mkCIdent `NFA.Checked.Transition.mk)
+                #[Quote.quote t.start, Quote.quote t.«end», Quote.quote t.next]
+
+instance : Quote (NFA.Checked.Transition n) where
+  quote := mkTermOfTransition
+
+private def mkTermOfLook (l : NFA.Look) : Term :=
+  match l with
+  | .Start => Syntax.mkApp (mkCIdent ``NFA.Look.Start) #[]
+  | .End => Syntax.mkApp (mkCIdent ``NFA.Look.End) #[]
+  | .StartLF => Syntax.mkApp (mkCIdent ``NFA.Look.StartLF) #[]
+  | .EndLF => Syntax.mkApp (mkCIdent ``NFA.Look.EndLF) #[]
+  | .StartCRLF => Syntax.mkApp (mkCIdent ``NFA.Look.StartCRLF) #[]
+  | .EndCRLF => Syntax.mkApp (mkCIdent ``NFA.Look.EndCRLF) #[]
+  | .WordUnicode => Syntax.mkApp (mkCIdent ``NFA.Look.WordUnicode) #[]
+  | .WordUnicodeNegate => Syntax.mkApp (mkCIdent ``NFA.Look.WordUnicodeNegate) #[]
+  | .WordStartUnicode => Syntax.mkApp (mkCIdent ``NFA.Look.WordStartUnicode) #[]
+  | .WordEndUnicode => Syntax.mkApp (mkCIdent ``NFA.Look.WordEndUnicode) #[]
+  | .WordStartHalfUnicode => Syntax.mkApp (mkCIdent ``NFA.Look.WordStartHalfUnicode) #[]
+  | .WordEndHalfUnicode => Syntax.mkApp (mkCIdent ``NFA.Look.WordEndHalfUnicode) #[]
+
+instance : Quote NFA.Look where
+  quote := mkTermOfLook
+
+private def mkTermOfState (s : NFA.Checked.State n) : Term :=
+  match s with
+  | .Empty next =>
+      Syntax.mkApp (mkCIdent ``NFA.Checked.State.Empty) #[Quote.quote next]
+  | .ByteRange t =>
+      Syntax.mkApp (mkCIdent ``NFA.Checked.State.ByteRange) #[Quote.quote t]
+  | .SparseTransitions transitions =>
+      Syntax.mkApp (mkCIdent ``NFA.Checked.State.SparseTransitions) #[Quote.quote transitions]
+  | .Look look next =>
+      Syntax.mkApp (mkCIdent ``NFA.Checked.State.Look) #[Quote.quote look, Quote.quote next]
+  | .Union alts =>
+      Syntax.mkApp (mkCIdent ``NFA.Checked.State.Union) #[Quote.quote alts]
+  | .UnionReverse alts =>
+      Syntax.mkApp (mkCIdent ``NFA.Checked.State.UnionReverse) #[Quote.quote alts]
+  | .BinaryUnion alt1 alt2 =>
+      Syntax.mkApp (mkCIdent ``NFA.Checked.State.BinaryUnion) #[Quote.quote alt1, Quote.quote alt2]
+  | .Capture next id g s =>
+      Syntax.mkApp (mkCIdent ``NFA.Checked.State.Capture)
+        #[Quote.quote next, toNumLit id, toNumLit g, toNumLit s]
+  | .Match id =>
+      Syntax.mkApp (mkCIdent ``NFA.Checked.State.Match) #[toNumLit id]
+
+instance : Quote (NFA.Checked.State n) where
+  quote := mkTermOfState
+
+/-- proof of `n` = `list.toArray.size`
+
+  for example:
+
+  @of_eq_true (1 = #[1].size) ((congrArg (Eq 1) (Array.size_toArray [1])).trans (eq_self 1))
+  : 1 = #[1].size
+
+-/
+private def mkTermIsEq (n : Nat) (list : Term) : Term :=
+  let mkTermEq :=
+        Syntax.mkApp (mkCIdent ``Eq) #[Lean.Syntax.mkNumLit (ToString.toString n)]
+
+  let mkTermEqSelf :=
+        Syntax.mkApp (mkCIdent ``eq_self) #[Lean.Syntax.mkNumLit (ToString.toString n)]
+
+  let mkTermSizeToArray :=
+      Syntax.mkApp (mkCIdent ``Array.size_toArray) #[list]
+
+  let mkTermCongrArg (f h : Term) :=
+        Syntax.mkApp (mkCIdent ``congrArg) #[f, h]
+
+  let mkTermEqTrans (h1 h2 : Term) :=
+        Syntax.mkApp (mkCIdent ``Eq.trans) #[h1, h2]
+
+  let mkTermOfEqTrue (h : Term) :=
+        Syntax.mkApp (mkCIdent ``of_eq_true) #[h]
+
+  mkTermOfEqTrue (mkTermEqTrans (mkTermCongrArg mkTermEq mkTermSizeToArray) mkTermEqSelf)
+
+private def mkTermOfNfa (nfa : NFA.Checked.NFA) : Term :=
+  let data : Term := Quote.quote nfa.states.data
+  let states : Term := Syntax.mkApp (mkCIdent `Array.mk) #[data]
+  Syntax.mkApp (mkCIdent `NFA.Checked.NFA.mk)
+      #[Lean.Syntax.mkNumLit (ToString.toString nfa.n), states, mkTermIsEq nfa.n data]
+
+private def mkTermOfRegex (re : Regex.Regex) : Term :=
+  Syntax.mkApp (mkCIdent `Regex.Regex.mk) #[mkTermOfNfa re.nfa]
+
+declare_syntax_cat regex
+syntax str : regex
+syntax "regex%" regex : term
+
+/-- build regular expressions at compile time -/
+macro_rules
+| `(regex% $p:str) =>
+    match Regex.build p.getString with
+    | Except.ok re => return mkTermOfRegex re
+    | Except.error e => throw <| Lean.Macro.Exception.error p e
